theories/Core/Utils.v
@@ -35,6 +35,23 @@ Ltac break :=
          end.
 
 (* A smarter version of this should be part of the [coinduction] library *)
+
+(* Ltac step := *)
+(*   match goal with *)
+(*   | |- gfp _ _ _ => tactics.step *)
+(*   | |- _ => red; tactics.step *)
+(*   end. *)
+Ltac step_ :=
+  match goal with
+  | |- gfp ?b ?x ?y => apply (proj2 (gfp_fp b x y))
+  | |- body (t ?b) ?R ?x ?y => apply (bt_t b R x y)
+  | |- gfp ?b ?x => apply (proj2 (gfp_fp b x))
+  | |- body (t ?b) ?R ?x => apply (bt_t b R x)
+  end;
+  simpl body.
+
+Ltac step := first [step_ | red; step_].
+
 Ltac step_in H :=
 match type of H with
 | gfp ?b ?x ?y => apply (gfp_fp b x y) in H
@@ -45,4 +62,3 @@ match type of H with
 end;
 simpl body in H.
 Tactic Notation "step" "in" ident(H) := step_in H.
-
