theories/Eq/Visible.v
@@ -1,0 +1,94 @@
+From RelationAlgebra Require Import
+     monoid
+     kat
+     kat_tac
+     prop
+     rel
+     srel
+     comparisons
+     rewriting
+     normalisation.
+
+From Coinduction Require Import
+	 coinduction rel tactics.
+
+From CTree Require Import
+	 CTree Eq.Shallow Eq.Equ.
+
+Import CTree.
+Import CTreeNotations.
+Import EquNotations.
+Open Scope ctree.
+
+Set Implicit Arguments.
+Set Primitive Projections.
+
+Section Visible.
+
+  Context {E : Type -> Type} {R : Type}.
+
+  Notation S' := (ctree' E R).
+  Notation S  := (ctree  E R).
+
+  Definition SS : EqType :=
+	{| type_of := S ; Eq := equ eq |}.
+
+  Inductive visible_ : hrel S' S' :=
+  | VisibleI {n} (x : Fin.t n) k t :
+    visible_ (observe (k x)) t ->
+    visible_ (ChoiceF false n k) t
+
+  | VisibleV {n} (x : Fin.t n) k1 k2 :
+    (forall x, k1 x ≅ k2 x) ->
+    visible_ (ChoiceF true n k1) (ChoiceF true n k2)
+
+  | VisibleVis {X} (e : E X) k1 k2 :
+    (forall x, k1 x ≅ k2 x) ->
+    visible_ (VisF e k1) (VisF e k2)
+
+  | VisibleRet r :
+    visible_ (RetF r) (RetF r)
+  .
+  Hint Constructors visible_ : core.
+
+  Definition visibleR : hrel S S :=
+	fun u v => visible_ (observe u) (observe v).
+
+  #[local] Instance visible__equ_aux1 t :
+	Proper (going (equ eq) ==> flip impl) (visible_ t).
+  Proof.
+	intros x x' equ TR.
+	inv equ; rename H into equ.
+	step in equ.
+	dependent induction TR; intros; eauto; inv equ; try invert; auto;
+	  (constructor; auto; etransitivity; [apply H | symmetry; auto]).
+  Qed.
+
+  #[local] Instance visible__equ_aux2 :
+	Proper (going (equ eq) ==> going (equ eq) ==> impl) visible_.
+  Proof.
+	intros x x' xequ y y' yequ TR. rewrite <- yequ. clear yequ y'.
+	inv xequ; rename H into xequ.	step in xequ.
+    revert x' xequ.
+	dependent induction TR; intros; eauto; inv xequ; try invert; auto.
+    2, 3: constructor; auto; intros; rewrite <- H; symmetry; auto.
+    econstructor. apply IHTR. rewrite REL. reflexivity.
+  Qed.
+
+  #[global] Instance visible__equ :
+	Proper (going (equ eq) ==> going (equ eq) ==> iff) visible_.
+  Proof.
+	intros ? ? eqt ? ? equ; split; intros TR.
+	- eapply visible__equ_aux2; eauto.
+	- symmetry in equ; symmetry in eqt; eapply visible__equ_aux2; eauto.
+  Qed.
+
+  #[global] Instance visible_equ :
+	Proper (equ eq ==> equ eq ==> iff) visibleR.
+  Proof.
+	intros ? ? eqt ? ? equ; unfold visibleR.
+    rewrite eqt, equ. reflexivity.
+  Qed.
+
+  Definition visible : srel SS SS := {| hrel_of := visibleR : hrel SS SS |}.
+End Visible.
